libcrux-iot/ml-kem/proofs/fstar/extraction/Libcrux_iot_ml_kem.Vector.Portable.Vector_type.fsti
@@ -24,7 +24,10 @@ val zero: Prims.unit -> Prims.Pure t_PortableVector Prims.l_True (fun _ -> Prims
 val to_i16_array (x: t_PortableVector) (out: t_Slice i16)
     : Prims.Pure (t_Slice i16)
       (requires (Core.Slice.impl__len #i16 out <: usize) =. mk_usize 16)
-      (fun _ -> Prims.l_True)
+      (ensures
+        fun out_future ->
+          let out_future:t_Slice i16 = out_future in
+          (Core.Slice.impl__len #i16 out_future <: usize) =. mk_usize 16)
 
 val from_i16_array (array: t_Slice i16) (out: t_PortableVector)
     : Prims.Pure t_PortableVector
