libcrux-iot/ml-kem/proofs/fstar/extraction/Libcrux_iot_ml_kem.Vector.Portable.fsti
@@ -7,11 +7,16 @@ let _ =
   (* This module has implicit dependencies, here we make them explicit. *)
   (* The implicit dependencies arise from typeclasses instances. *)
   let open Libcrux_iot_ml_kem.Vector.Portable.Vector_type in
+  let open Libcrux_iot_ml_kem.Vector.Traits in
   let open Libcrux_secrets.Int.Classify_public in
   let open Libcrux_secrets.Int.Public_integers in
   let open Libcrux_secrets.Traits in
   ()
 
 [@@ FStar.Tactics.Typeclasses.tcinstance]
-val impl:Libcrux_iot_ml_kem.Vector.Traits.t_Operations
+val impl:Libcrux_iot_ml_kem.Vector.Traits.t_Repr
+Libcrux_iot_ml_kem.Vector.Portable.Vector_type.t_PortableVector
+
+[@@ FStar.Tactics.Typeclasses.tcinstance]
+val impl_1:Libcrux_iot_ml_kem.Vector.Traits.t_Operations
 Libcrux_iot_ml_kem.Vector.Portable.Vector_type.t_PortableVector
