libcrux-iot/ml-kem/proofs/fstar/extraction/Libcrux_iot_ml_kem.Vector.Traits.Spec.fst
@@ -69,6 +69,15 @@ let montgomery_multiply_by_constant_post
   Spec.Utils.is_i16b_array 3328 result /\
   (forall i. ((v (Seq.index result i) % 3329) == (v (Seq.index vec i) * v c * 169) % 3329))
 
+let to_unsigned_representative_pre (vec: t_Array i16 (mk_usize 16)) : Hax_lib.Prop.t_Prop =
+  Spec.Utils.is_i16b_array 3328 vec
+
+let to_unsigned_representative_post (vec result: t_Array i16 (mk_usize 16)) : Hax_lib.Prop.t_Prop =
+  forall i.
+    let x = Seq.index vec i in
+    let y = Seq.index result i in
+    (v y >= 0 /\ v y <= 3328 /\ (v y % 3329 == v x % 3329))
+
 let compress_1_pre (vec: t_Array i16 (mk_usize 16)) : Hax_lib.Prop.t_Prop =
   forall i. v (Seq.index vec i) >= 0 /\ v (Seq.index vec i) < 3329
 
@@ -88,8 +97,140 @@ let compress_post
     v coefficient_bits == 11) ==>
   (forall i. bounded (Seq.index result i) (v coefficient_bits))
 
+let decompress_1_pre (vec: t_Array i16 (mk_usize 16)) : Hax_lib.Prop.t_Prop =
+  forall i.
+    let x = Seq.index vec i in
+    (x == mk_i16 0 \/ x == mk_i16 1)
+
 let decompress_ciphertext_coefficient_pre (vec: t_Array i16 (mk_usize 16)) (coefficient_bits: i32)
     : Hax_lib.Prop.t_Prop =
   (v coefficient_bits == 4 \/ v coefficient_bits == 5 \/ v coefficient_bits == 10 \/
     v coefficient_bits == 11) /\
   (forall i. v (Seq.index vec i) >= 0 /\ v (Seq.index vec i) < pow2 (v coefficient_bits))
+
+let ntt_layer_1_step_pre (vec: t_Array i16 (mk_usize 16)) (zeta0 zeta1 zeta2 zeta3: i16)
+    : Hax_lib.Prop.t_Prop =
+  Spec.Utils.is_i16b 1664 zeta0 /\ Spec.Utils.is_i16b 1664 zeta1 /\ Spec.Utils.is_i16b 1664 zeta2 /\
+  Spec.Utils.is_i16b 1664 zeta3 /\ Spec.Utils.is_i16b_array (11207 + 5 * 3328) vec
+
+let ntt_layer_1_step_post
+      (vec: t_Array i16 (mk_usize 16))
+      (zeta0 zeta1 zeta2 zeta3: i16)
+      (result: t_Array i16 (mk_usize 16))
+    : Hax_lib.Prop.t_Prop = Spec.Utils.is_i16b_array (11207 + 6 * 3328) result
+
+let ntt_layer_2_step_pre (vec: t_Array i16 (mk_usize 16)) (zeta0 zeta1: i16) : Hax_lib.Prop.t_Prop =
+  Spec.Utils.is_i16b 1664 zeta0 /\ Spec.Utils.is_i16b 1664 zeta1 /\
+  Spec.Utils.is_i16b_array (11207 + 4 * 3328) vec
+
+let ntt_layer_2_step_post
+      (vec: t_Array i16 (mk_usize 16))
+      (zeta0 zeta1: i16)
+      (result: t_Array i16 (mk_usize 16))
+    : Hax_lib.Prop.t_Prop = Spec.Utils.is_i16b_array (11207 + 5 * 3328) result
+
+let ntt_layer_3_step_pre (vec: t_Array i16 (mk_usize 16)) (zeta0: i16) : Hax_lib.Prop.t_Prop =
+  Spec.Utils.is_i16b 1664 zeta0 /\ Spec.Utils.is_i16b_array (11207 + 3 * 3328) vec
+
+let ntt_layer_3_step_post
+      (vec: t_Array i16 (mk_usize 16))
+      (zeta0: i16)
+      (result: t_Array i16 (mk_usize 16))
+    : Hax_lib.Prop.t_Prop = Spec.Utils.is_i16b_array (11207 + 4 * 3328) result
+
+let inv_ntt_layer_1_step_pre (vec: t_Array i16 (mk_usize 16)) (zeta0 zeta1 zeta2 zeta3: i16)
+    : Hax_lib.Prop.t_Prop =
+  Spec.Utils.is_i16b 1664 zeta0 /\ Spec.Utils.is_i16b 1664 zeta1 /\ Spec.Utils.is_i16b 1664 zeta2 /\
+  Spec.Utils.is_i16b 1664 zeta3 /\ Spec.Utils.is_i16b_array (4 * 3328) vec
+
+let inv_ntt_layer_1_step_post
+      (vec: t_Array i16 (mk_usize 16))
+      (zeta0 zeta1 zeta2 zeta3: i16)
+      (result: t_Array i16 (mk_usize 16))
+    : Hax_lib.Prop.t_Prop = Spec.Utils.is_i16b_array 3328 result
+
+let inv_ntt_layer_2_step_pre (vec: t_Array i16 (mk_usize 16)) (zeta0 zeta1: i16)
+    : Hax_lib.Prop.t_Prop =
+  Spec.Utils.is_i16b 1664 zeta0 /\ Spec.Utils.is_i16b 1664 zeta1 /\
+  Spec.Utils.is_i16b_array 3328 vec
+
+let inv_ntt_layer_2_step_post
+      (vec: t_Array i16 (mk_usize 16))
+      (zeta0 zeta1: i16)
+      (result: t_Array i16 (mk_usize 16))
+    : Hax_lib.Prop.t_Prop = Spec.Utils.is_i16b_array 3328 result
+
+let inv_ntt_layer_3_step_pre (vec: t_Array i16 (mk_usize 16)) (zeta0: i16) : Hax_lib.Prop.t_Prop =
+  Spec.Utils.is_i16b 1664 zeta0 /\ Spec.Utils.is_i16b_array 3328 vec
+
+let inv_ntt_layer_3_step_post
+      (vec: t_Array i16 (mk_usize 16))
+      (zeta0: i16)
+      (result: t_Array i16 (mk_usize 16))
+    : Hax_lib.Prop.t_Prop = Spec.Utils.is_i16b_array 3328 result
+
+let ntt_multiply_pre (lhs rhs out: t_Array i16 (mk_usize 16)) (zeta0 zeta1 zeta2 zeta3: i16)
+    : Hax_lib.Prop.t_Prop =
+  Spec.Utils.is_i16b 1664 zeta0 /\ Spec.Utils.is_i16b 1664 zeta1 /\ Spec.Utils.is_i16b 1664 zeta2 /\
+  Spec.Utils.is_i16b 1664 zeta3 /\ Spec.Utils.is_i16b_array 3328 lhs /\
+  Spec.Utils.is_i16b_array 3328 rhs
+
+let ntt_multiply_post
+      (lhs rhs out: t_Array i16 (mk_usize 16))
+      (zeta0 zeta1 zeta2 zeta3: i16)
+      (result: t_Array i16 (mk_usize 16))
+    : Hax_lib.Prop.t_Prop = Spec.Utils.is_i16b_array 3328 result
+
+let serialize_1_pre (vec: t_Array i16 (mk_usize 16)) (out: t_Slice u8) : Hax_lib.Prop.t_Prop =
+  Seq.length out == 2 /\ Spec.MLKEM.serialize_pre 1 vec
+
+let serialize_1_post (vec: t_Array i16 (mk_usize 16)) (out result: t_Slice u8) : Hax_lib.Prop.t_Prop =
+  Seq.length result == 2 /\
+  (Spec.MLKEM.serialize_pre 1 vec ==> Spec.MLKEM.serialize_post 1 vec result)
+
+let deserialize_1_pre (input: t_Slice u8) (out: t_Array i16 (mk_usize 16)) : Hax_lib.Prop.t_Prop =
+  Seq.length input == 2
+
+let deserialize_1_post (input: t_Slice u8) (out result: t_Array i16 (mk_usize 16))
+    : Hax_lib.Prop.t_Prop = Seq.length input == 2 ==> Spec.MLKEM.deserialize_post 1 input result
+
+let serialize_4_pre (vec: t_Array i16 (mk_usize 16)) (out: t_Slice u8) : Hax_lib.Prop.t_Prop =
+  Seq.length out == 8 /\ Spec.MLKEM.serialize_pre 4 vec
+
+let serialize_4_post (vec: t_Array i16 (mk_usize 16)) (out result: t_Slice u8) : Hax_lib.Prop.t_Prop =
+  Seq.length result == 8 /\
+  (Spec.MLKEM.serialize_pre 4 vec ==> Spec.MLKEM.serialize_post 4 vec result)
+
+let deserialize_4_pre (input: t_Slice u8) (out: t_Array i16 (mk_usize 16)) : Hax_lib.Prop.t_Prop =
+  Seq.length input == 8
+
+let deserialize_4_post (input: t_Slice u8) (out result: t_Array i16 (mk_usize 16))
+    : Hax_lib.Prop.t_Prop = Seq.length input == 8 ==> Spec.MLKEM.deserialize_post 4 input result
+
+let serialize_10_pre (vec: t_Array i16 (mk_usize 16)) (out: t_Slice u8) : Hax_lib.Prop.t_Prop =
+  Seq.length out == 20 /\ Spec.MLKEM.serialize_pre 10 vec
+
+let serialize_10_post (vec: t_Array i16 (mk_usize 16)) (out result: t_Slice u8)
+    : Hax_lib.Prop.t_Prop =
+  Seq.length result == 20 /\
+  (Spec.MLKEM.serialize_pre 10 vec ==> Spec.MLKEM.serialize_post 10 vec result)
+
+let deserialize_10_pre (input: t_Slice u8) (out: t_Array i16 (mk_usize 16)) : Hax_lib.Prop.t_Prop =
+  Seq.length input == 20
+
+let deserialize_10_post (input: t_Slice u8) (out result: t_Array i16 (mk_usize 16))
+    : Hax_lib.Prop.t_Prop = Seq.length input == 20 ==> Spec.MLKEM.deserialize_post 10 input result
+
+let serialize_12_pre (vec: t_Array i16 (mk_usize 16)) (out: t_Slice u8) : Hax_lib.Prop.t_Prop =
+  Seq.length out == 24 /\ Spec.MLKEM.serialize_pre 12 vec
+
+let serialize_12_post (vec: t_Array i16 (mk_usize 16)) (out result: t_Slice u8)
+    : Hax_lib.Prop.t_Prop =
+  Seq.length result == 24 /\
+  (Spec.MLKEM.serialize_pre 12 vec ==> Spec.MLKEM.serialize_post 12 vec result)
+
+let deserialize_12_pre (input: t_Slice u8) (out: t_Array i16 (mk_usize 16)) : Hax_lib.Prop.t_Prop =
+  Seq.length input == 24
+
+let deserialize_12_post (input: t_Slice u8) (out result: t_Array i16 (mk_usize 16))
+    : Hax_lib.Prop.t_Prop = Seq.length input == 24 ==> Spec.MLKEM.deserialize_post 12 input result
